From40To50/Proto.v
@@ -1,7 +1,8 @@
 From Coq Require Import String.
 
-From Vyper.L50 Require Import Types.
-From Vyper Require Import Config ProtoAST.
+From Vyper.L10 Require Import Base.
+From Vyper.L50 Require Import Types Builtins.
+From Vyper Require Import Config ProtoAST NaryFun.
 
 Local Open Scope list_scope.
 Local Open Scope string_scope.
@@ -66,3 +67,58 @@ Definition make_proto_table {C: VyperConfig} (asts: list proto_ast)
                       end
           end
    in add_protos asts Map.empty.
+
+(** Test if the only input and output type is u256 (or address, as we don't distinguish it from u256). *)
+Definition proto_is_u256_only (p: proto)
+: bool
+:= all_are_u256 (p_inputs p) && all_are_u256 (p_outputs p).
+
+(** Compile-time builtin function prototypes correspond with what the L50 interpreter got at runtime. *)
+Definition ProtosAgree {C: VyperConfig}
+                       (protos: string -> option proto)
+                       (builtins: string -> option L50.Builtins.yul_builtin)
+:= forall name,
+     match protos name, builtins name with
+     | None, None => True
+     | Some p, Some b => p_inputs p = L50.Builtins.b_input_types b 
+                          /\
+                         p_outputs p = L50.Builtins.b_output_types b
+     | _, _ => False
+     end.
+
+Definition call_builtin_u256 {C: VyperConfig}
+                             (b: yul_builtin)
+                             (world: world_state)
+                             (args: list uint256)
+                             (LenOk: List.length (b_input_types b) = List.length args)
+: world_state * expr_result (list uint256)
+:= fst (nary_call (b_fun b world) args (PeanoNat.Nat.eq_le_incl _ _ LenOk)).
+
+
+(*
+Definition call_builtin_on_u256_inputs {C: VyperConfig}
+                                       (b: yul_builtin)
+                                       (world: world_state)
+                                       (args: list uint256)
+                                       (LenOk: List.length (b_input_types b) = List.length args)
+: world_state * expr_result (list dynamic_value)
+:= match nary_call (b_fun b world) args (PeanoNat.Nat.eq_le_incl _ _ LenOk) with
+   | ((world', ExprSuccess outputs_256), _) =>
+       (world', match mass_cast outputs_256 (b_output_types b) with
+                | inl err => expr_error err
+                | inr outputs => ExprSuccess outputs
+                end)
+   | ((world', ExprAbort ab), _) => (world', ExprAbort ab)
+   end.
+
+Lemma call_builtin_on_u256_inputs_ok {C: VyperConfig}
+                                     (b: yul_builtin)
+                                     (world: world_state)
+                                     (args: list uint256)
+                                     (LenOk: List.length (b_input_types b) = List.length args)
+                                     (ArgTypesOk: all_are_u256 (b_input_types b) = true):
+  call_builtin_on_u256_inputs b world args ArgTypesOk LenOk
+   =
+  call_builtin b world (List.map (fun x => existT _ U256 (yul_uint256 x)) args).
+Proof.
+*)
